\section{Exercise 3}
Given formulas are:\\
\begin{center}
    \begin{equation}
        \frac{1}{\sigma^{2}_{n}}=\frac{n}{\sigma^{2}}+\frac{1}{\sigma^{2}_{0}}
        \label{eq:sigma}
    \end{equation}
\end{center}
\begin{center}
    \begin{equation}
        \frac{\mu_{n}}{\sigma^{2}_{n}}=\frac{n}{\sigma^{2}_{n}}\hat{\mu}_{n}+\frac{\mu_{0}}{\sigma^{2}_{0}}
    \end{equation}
\end{center}
\begin{center}
    \begin{equation}
        \hat{\mu}_{n}=\frac{1}{n}\sum_{k=1}^{n}x_{k}
    \end{equation}
\end{center}


\subsection{a}
We want to show that following relation holds:

\begin{center}
    \begin{equation}
        \sigma^{2}_{n}\le min\left(\frac{\sigma^{2}}{n},\sigma^{2}_{0}\right)
    \label{eq:3a}
    \end{equation}
\end{center}

At first we need a expression for $\sigma^{2}_{n}$. This will give us formula (\ref{eq:sigma}):

\begin{align*}
    &\Rightarrow&\frac{1}{\sigma^{2}_{n}} &=\frac{n}{\sigma^{2}}+\frac{1}{\sigma^{2}_{0}}\\
    &\Leftrightarrow& 1 &=\left(\frac{n}{\sigma^{2}}+\frac{1}{\sigma^{2}_{0}}\right)\cdot\sigma^{2}_{n}\\
    &\Leftrightarrow& \sigma^{2}_{n} &=\frac{1}{\frac{n}{\sigma^{2}}+\frac{1}{\sigma^{2}_{0}}}\\
    &\Leftrightarrow& \sigma^{2}_{n} &=\frac{1}{\frac{n\sigma^{^2}_{0}}{\sigma^{2}\sigma^{^2}_{0}}+\frac{\sigma^{2}}{\sigma^{2}_{0}\sigma^{2}}}\\
    &\Leftrightarrow& \sigma^{2}_{n} &=\frac{1}{\frac{n\sigma^{^2}_{0}+\sigma^{2}}{\sigma^2\sigma^{2}_{0}}}\\
    &\Leftrightarrow& \sigma^{2}_{n} &=\frac{\sigma^2\sigma^{2}_{0}}{n\sigma^{^2}_{0}+\sigma^{2}}
\end{align*}

Now we have two cases to consider to show that $\sigma^{2}_{n}\le min\left(\frac{\sigma^{2}}{n},\sigma^{2}_{0}\right)$ holds:
\begin{align}
    \text{case 1: } \sigma^{2}_{0}&\le\frac{\sigma^{2}}{n}\\
    \text{case 2: } \sigma^{2}_{0}&\ge\frac{\sigma^{2}}{n}
\end{align}

At first we take a look at case one:\\

\begin{align*}
    &\Rightarrow&\sigma^{2}_{n}&\le min\left(\frac{\sigma^{2}}{n},\sigma^{2}_{0}\right)\\
    &\Leftrightarrow&\sigma^{2}_{n}&\le\frac{\sigma^{2}}{n}\\
    &\Leftrightarrow& \frac{\sigma^2\sigma^{2}_{0}}{n\sigma^{^2}_{0}+\sigma^{2}} &\le\frac{\sigma^{2}}{n}\\
    &\Leftrightarrow& \frac{\sigma^{2}_{0}}{n\sigma^{^2}_{0}+\sigma^{2}} &\le\frac{1}{n}\\
    &\Leftrightarrow& \frac{1}{n\sigma^{^2}_{0}+\sigma^{2}} &\le\frac{1}{n\sigma^{2}_{0}}\\
    &\Leftrightarrow& 1 &\le\frac{n\sigma^{^2}_{0}+\sigma^{2}}{n\sigma^{2}_{0}}\\
    &\Leftrightarrow& 1 &\le 1+\frac{\sigma}{n\sigma^{2}_{0}}\\
    &\Leftrightarrow& 0 &\le \frac{\sigma}{n\sigma^{2}_{0}}
\end{align*}

This expression is true because $\sigma$, n and $\sigma_{0}$ are always greater than zero (or maybe sometimes equal to zero) and so we have shown thas the first case is true.\\
Now we take a look at case two:

\begin{align*}
    &\Rightarrow&\sigma^{2}_{n}&\le min\left(\frac{\sigma^{2}}{n},\sigma^{2}_{0}\right)\\
    &\Leftrightarrow&\sigma^{2}_{n}&\le\sigma^{2}_{0}\\
    &\Leftrightarrow& \frac{\sigma^2\sigma^{2}_{0}}{n\sigma^{^2}_{0}+\sigma^{2}} &\le\sigma^{2}_{0}\\
    &\Leftrightarrow& \frac{\sigma^2}{n\sigma^{^2}_{0}+\sigma^{2}} &\le 1\\
    &\Leftrightarrow&\sigma^2&\le n\sigma^{^2}_{0}+\sigma^{2}\\
    &\Leftrightarrow& 1\le\frac{n\sigma^{2}_{0}}{\sigma^{2}}-1\\
    &\Leftrightarrow& 0\le\frac{n\sigma^{2}_{0}}{\sigma^{2}}
\end{align*}

Like in case one is this expression true because $\sigma$, n and $\sigma_{0}$ are always greater than zero (or maybe sometimes equal to zero) and so we have shown thas the second case is true.\\
So we have shown that relation (\ref{eq:3a}) holds.

\subsection*{3b}
Prove that $min(\hat{\mu}_n, \mu_0)\leq \mu_n \leq max(\hat{\mu}_n, \mu_0)$
\begin{align*}
   \frac{\mu_n}{\sigma^{2}_{n}} &= \frac{n}{\sigma^{2}}\hat{\mu}_n+\frac{\mu_0}{\sigma^{2}_0}\\
   \Leftrightarrow\frac{\mu_n}{\frac{\sigma^2\sigma^{2}_{0}}{n\sigma^{^2}_{0}+\sigma^{2}}} &= \frac{n}{\sigma^{2}}\hat{\mu}_n+\frac{\mu_0}{\sigma^{2}_0}\\
   \Leftrightarrow \mu_n&=\frac{n\sigma^{2}_0\hat{\mu}_n + \mu_0\sigma^{^2}}{n\sigma^{^2}_{0}+\sigma^{2}}
\end{align*}
\hspace*{2mm}If $\hat{\mu}_n \leq \mu_n$:
\begin{align*}
\hat{\mu}_n &\leq\frac{n\sigma^{2}_0\hat{\mu}_n + \mu_0\sigma^{^2}}{n\sigma^{^2}_{0}+\sigma^{2}}\\
\Leftrightarrow0&\leq\frac{n\sigma^{2}_0\hat{\mu}_n + \mu_0\sigma^{^2}-\hat{\mu}_n(n\sigma^{^2}_{0}+\sigma^{2})}{n\sigma^{^2}_{0}+\sigma^{2}}\\
\Leftrightarrow0&\leq\frac{\mu_0\sigma^{2}-\hat{\mu}_n\sigma^{2}}{n\sigma^{^2}_{0}+\sigma^{2}}\\
\Leftrightarrow 0&\leq \sigma^{2}(\mu_0-\hat{\mu}_n),\ because\ neither\ n,\ \sigma^{^2}_{0}\ or\ \sigma^{2}\ can\ be\ negative\\
\Leftrightarrow 0&\leq \mu_0-\hat{\mu}_n,\ because\ \sigma^{2}>0\\
\Leftrightarrow \hat{\mu}_n&\leq \mu_0
\end{align*}
\hspace{10mm}If $\hat{\mu}_n \leq \mu_n ,\ \mu_0$ has to be greater or equals to $\mu_n$ to fulfill \\\hspace*{10mm}$min(\hat{\mu}_n, \mu_0)\leq \mu_n \leq max(\hat{\mu}_n, \mu_0)$ because of transitivity\\ 
\hspace*{10mm}that would mean $\hat{\mu}_n\leq \mu_0$ is true.\\ \\
\hspace*{5mm}Test whether $\mu_0\geq \mu_n$ if $\hat{\mu}_n \leq \mu_n$:
\begin{align*}
    \mu_0&\geq \mu_n \\
    \Leftrightarrow \mu_0&\geq\frac{n\sigma^{2}_0\hat{\mu}_n + \mu_0\sigma^{^2}}{n\sigma^{^2}_{0}+\sigma^{2}}\\
    \Leftrightarrow 0&\geq\frac{n\sigma^{2}_0\hat{\mu}_n + \mu_0\sigma^{^2}-\mu_0(n\sigma^{^2}_{0}+\sigma^{2})}{n\sigma^{^2}_{0}+\sigma^{2}}\\
    \Leftrightarrow 0&\geq\frac{n\sigma^{2}_0\hat{\mu}_n -\mu_0n\sigma^{^2}_{0}}{n\sigma^{2}_{0}+\sigma^{2}}\\
    \Leftrightarrow 0&\geq n\sigma^{2}_0\hat{\mu}_n -\mu_0n\sigma^{2}_{0},\ because\ n,\ \sigma^{2}_{0}\ and\  \sigma^{2}>0\\
    \Leftrightarrow \mu_0&\geq \hat{\mu}_n
\end{align*}
\hspace*{5mm}$\Rightarrow$ If $\mu_0\geq \hat{\mu}_n$ then $min(\hat{\mu}_n, \mu_0)\leq \mu_n \leq max(\hat{\mu}_n, \mu_0)$ is true.\\ \\
\hspace*{2mm} Same can be proven for $\hat{\mu}_n \geq \mu_n$:
\begin{align*}
\hat{\mu}_n &\geq\frac{n\sigma^{2}_0\hat{\mu}_n + \mu_0\sigma^{^2}}{n\sigma^{^2}_{0}+\sigma^{2}}\\
\Leftrightarrow0&\geq\frac{n\sigma^{2}_0\hat{\mu}_n + \mu_0\sigma^{^2}-\hat{\mu}_n(n\sigma^{^2}_{0}+\sigma^{2})}{n\sigma^{^2}_{0}+\sigma^{2}}\\
\Leftrightarrow0&\geq\frac{\mu_0\sigma^{2}-\hat{\mu}_n\sigma^{2}}{n\sigma^{^2}_{0}+\sigma^{2}}\\
\Leftrightarrow 0&\geq \sigma^{2}(\mu_0-\hat{\mu}_n),\ because\ neither\ n,\ \sigma^{^2}_{0}\ or\ \sigma^{2}\ can\ be\ negative\\
\Leftrightarrow 0&\geq \mu_0-\hat{\mu}_n,\ because\ \sigma^{2}>0\\
\Leftrightarrow \hat{\mu}_n&\geq \mu_0
\end{align*}
\hspace*{5mm}Test whether $\mu_n\geq \mu_0$ if $\hat{\mu}_n \geq \mu_n$:
\begin{align*}
    \mu_0&\leq \mu_n \\
    \Leftrightarrow \mu_0&\leq\frac{n\sigma^{2}_0\hat{\mu}_n + \mu_0\sigma^{^2}}{n\sigma^{^2}_{0}+\sigma^{2}}\\
    \Leftrightarrow 0&\leq\frac{n\sigma^{2}_0\hat{\mu}_n + \mu_0\sigma^{^2}-\mu_0(n\sigma^{^2}_{0}+\sigma^{2})}{n\sigma^{^2}_{0}+\sigma^{2}}\\
    \Leftrightarrow 0&\leq\frac{n\sigma^{2}_0\hat{\mu}_n -\mu_0n\sigma^{^2}_{0}}{n\sigma^{2}_{0}+\sigma^{2}}\\
    \Leftrightarrow 0&\leq n\sigma^{2}_0\hat{\mu}_n -\mu_0n\sigma^{2}_{0},\ because\ n,\ \sigma^{2}_{0}\ and\  \sigma^{2}>0\\
    \Leftrightarrow \mu_0&\leq \hat{\mu}_n
\end{align*}
\hspace*{5mm}$\Rightarrow$ If $\hat{\mu}_n\geq \mu_n$ then $min(\hat{\mu}_n, \mu_0)\leq \mu_n \leq max(\hat{\mu}_n, \mu_0)$ is true.\\ \\
It is proven that $min(\hat{\mu}_n, \mu_0)\leq \mu_n \leq max(\hat{\mu}_n, \mu_0)$